Additional backend support (#6)
* trait issue

* remove trait file

* backends

Library/DRandom.cs
@@ -1,0 +1,22 @@
+/*******************************************************************************
+*  Copyright by the contributors to the Dafny Project
+*  SPDX-License-Identifier: MIT
+*******************************************************************************/
+
+using System;
+
+namespace DafnyLibraries {
+  public partial class DRandom : DRandomTrait {
+    private Random r;
+
+    public DRandom() {
+      this.r = new Random();
+    }
+
+    public bool Coin() {
+      return this.r.Next(2) == 0;
+    }
+  }
+}
+
+
