Library/DRandom.go
@@ -1,0 +1,19 @@
+/*******************************************************************************
+*  Copyright by the contributors to the Dafny Project
+*  SPDX-License-Identifier: MIT
+*******************************************************************************/
+
+package DafnyLibraries
+
+import(
+  "math/rand"
+)
+
+func *DRandom Ctor__(self) {
+}
+
+func *DRandom Coin() bool {
+  return rand.Intn(2)
+}
+
+
