Library/DRandom.js
@@ -1,0 +1,17 @@
+/*******************************************************************************
+*  Copyright by the contributors to the Dafny Project
+*  SPDX-License-Identifier: MIT
+*******************************************************************************/
+
+
+let DafnyLibraries = (function() {
+  let $module = {};
+
+  $module.DRandom = class DRandom {
+    constructor() { }
+
+    Coin() {
+      return Boolean(Math.random() < 0.5);
+    }
+  };
+})();
