Library/DRandom.dfy
@@ -8,30 +8,59 @@
 include "Model/RandomNumberGenerator.dfy"
 include "Model/Model.dfy"
 include "Model/Monad.dfy"
-include "RandomTrait.dfy"
 include "Model/Bernoulli.dfy"
 include "Model/Uniform.dfy"
 
 module {:extern "DafnyLibraries"} DafnyLibraries {
-  import opened RandomTrait
   import opened RandomNumberGenerator
   import opened Monad
   import opened Bernoulli
   import opened Unif = Uniform
-  import Model
+  import opened Model
 
-  class {:extern} Random extends RandomTrait {
+  // Only here because of #2500. Should really be imported from separate file.
+  trait DRandomTrait {
+    ghost var s: RNG
+
+    method Coin() returns (b: bool)
+      modifies this
+      ensures CoinModel(old(s)) == (b, s)
+  //  ensures forall b :: mu(iset s | Model.Coin(s).0 == b) == 0.5
+
+    method Uniform(n: nat) returns (u: nat)
+      modifies this
+      requires 0 < n
+      ensures UniformModel(n)(old(s)) == (u, s)
+      decreases *
+  //  ensures forall i | 0 <= i < n :: mu(iset s | Model.Uniform(n)(s).0 == i) == 1.0 / (n as real)
+
+    method UniformInterval(a: int, b: int) returns (u: int)
+      modifies this
+      requires a < b
+      ensures UniformIntervalModel(a, b)(old(s)) == (u, s)
+      decreases *
+  //  ensures forall i | a <= i < b :: mu(iset s | Model.UniformInterval(a, b)(s).0 == i) == 1.0 / ((b - a) as real)
+
+    method Bernoulli(p: real) returns (c: bool) 
+      modifies this
+      decreases *            
+      requires 0.0 <= p <= 1.0
+      ensures BernoulliModel(p)(old(s)) == (c, s) 
+  //  ensures mu(iset s | Model.Bernoulli(p)(s).0) == p
+  }
+
+  class {:extern} DRandom extends DRandomTrait {
     constructor {:extern} ()
     
     method {:extern} Coin() returns (b: bool)
       modifies this
-      ensures Model.Coin(old(s)) == (b, s)
+      ensures CoinModel(old(s)) == (b, s)
 
     // Based on https://arxiv.org/pdf/1304.1916.pdf; unverified.
     method Uniform(n: nat) returns (u: nat)
       modifies this
       requires 0 < n
-      ensures Model.Uniform(n)(old(s)) == (u, s)
+      ensures UniformModel(n)(old(s)) == (u, s)
       decreases *
     {
       assume {:axiom} false;
@@ -55,12 +84,12 @@ module {:extern "DafnyLibraries"} DafnyLibraries {
     method UniformInterval(a: int, b: int) returns (u: int)
       modifies this
       requires a < b
-      ensures Model.UniformInterval(a, b)(old(s)) == (u, s)
+      ensures UniformIntervalModel(a, b)(old(s)) == (u, s)
       decreases *
     {
       var v := Uniform(b - a);
-      assert Model.Uniform(b-a)(old(s)) == (v, s);
-      assert Model.UniformInterval(a, b)(old(s)) == (a + v, s);
+      assert UniformModel(b-a)(old(s)) == (v, s);
+      assert UniformIntervalModel(a, b)(old(s)) == (a + v, s);
       u := a + v;
     }
 
@@ -68,7 +97,7 @@ module {:extern "DafnyLibraries"} DafnyLibraries {
       modifies this 
       decreases *
       requires 0.0 <= p <= 1.0
-      ensures Model.Bernoulli(p)(old(s)) == (c, s)
+      ensures BernoulliModel(p)(old(s)) == (c, s)
     {
       var q: Probability := p as real;
 
@@ -88,7 +117,7 @@ module {:extern "DafnyLibraries"} DafnyLibraries {
       }
 
       while true
-        invariant Model.Bernoulli(p)(old(s)) == Model.Bernoulli(q)(s)
+        invariant BernoulliModel(p)(old(s)) == BernoulliModel(q)(s)
         decreases *
       {
         b := Coin();
